src/Raft.thy
@@ -59,199 +59,104 @@ lemma (in raft)
   assumes "number_of_nodes = 3"
   obtains \<sigma> ms where "(hd all_states, hd all_messages) \<rightarrow>* (\<sigma>, ms)" "state (\<sigma> ! 0) = leader"
 proof-
-  have "([initial_server_state 3, initial_server_state 3, initial_server_state 3], hd all_messages)
-    \<rightarrow>* ([initial_server_state 3 \<lparr>currentTerm := increment_election_term (currentTerm (hd all_states ! 0)), votedFor := Some (node 0)\<rparr>, initial_server_state 3, initial_server_state 3],
-    {
-      message (node 0) (node 1) (request_vote (node 0) (log_index 0) (election_term 0)) (election_term 1),
-      message (node 0) (node 2) (request_vote (node 0) (log_index 0) (election_term 0)) (election_term 1)
-    })"
+  have "(hd all_states, hd all_messages) = (repeat (initial_server_state 3) 3, {})"
+    by (simp add: assms initial_state initial_message)
+  also have "\<dots> \<rightarrow>*
+    ([initial_server_state 3 \<lparr>currentTerm := increment_election_term (currentTerm (initial_server_state 3)), votedFor := Some (node 0)\<rparr>, initial_server_state 3, initial_server_state 3],
+    {message (node 0) (node 1) (request_vote (node 0) (log_index 0) (election_term 0)) (election_term 1),message (node 0) (node 2) (request_vote (node 0) (log_index 0) (election_term 0)) (election_term 1)})"
     apply (rule transitions_one)
-    apply (cut_tac TR_start_election
-        [where ms = "hd all_messages"
-          , where \<sigma> = "[initial_server_state 3, initial_server_state 3, initial_server_state 3]"
-          ])
-    apply simp_all
-    defer
-    apply (simp add: initial_server_state_def)
+    apply (rule TR_start_election [where target = 0])
+    apply (simp add: TR_condition_start_election_def)
+    apply (auto simp add: initial_server_state_def repeat_length numeral_3_eq_3)
+    done
+  also have "\<dots> \<rightarrow>* (
+    [initial_server_state 3 \<lparr>currentTerm := increment_election_term (currentTerm (initial_server_state 3)), votedFor := Some (node 0)\<rparr>,initial_server_state 3 \<lparr>votedFor := Some (node 0)\<rparr>, initial_server_state 3],
+    {message (node 1) (node 0) (request_vote_response True) (election_term 1),message (node 0) (node 1) (request_vote (node 0) (log_index 0) (election_term 0)) (election_term 1),message (node 0) (node 2) (request_vote (node 0) (log_index 0) (election_term 0)) (election_term 1)})"
+    apply (rule transitions_one)
+    apply (rule TR_request_vote_resp [where m = 1, where r = 0, where vg = True, where t = "election_term 1", where s = "node 0"])
+    apply (simp add: TR_condition_request_vote_resp_def)
   proof-
-    assume "([initial_server_state 3, initial_server_state 3, initial_server_state 3], hd all_messages) \<rightarrow>
-    ([initial_server_state 3\<lparr>currentTerm := election_term (Suc (election_term_of (currentTerm (initial_server_state 3)))), votedFor := Some (node 0)\<rparr>,
-      initial_server_state 3, initial_server_state 3],
-     hd all_messages \<union>
-     {message (node 0) (node i) (request_vote (node 0) (log_index 0) (election_term 0))
-       (election_term (Suc (election_term_of (currentTerm (initial_server_state 3))))) |
-      i. i \<le> Suc (Suc 0) \<and> 0 < i})"
+    have "ExReqProps (message (node (Suc 0)) (node 0) (request_vote_response True) (election_term (Suc 0)))
+        (\<lambda>req. \<not> sender_term req < election_term (Suc (election_term_of (currentTerm (initial_server_state 3)))) \<and>
+                (\<not> sender_term req < election_term (Suc (election_term_of (currentTerm (initial_server_state 3)))) \<longrightarrow>
+                 (\<exists>lastLogIndex lastLogTerm.
+                     payload req = request_vote (node 0) lastLogIndex lastLogTerm \<and>
+                     (req = message (node 0) (node (Suc 0)) (request_vote (node 0) (log_index 0) (election_term 0)) (election_term (Suc 0)) \<or>
+                      req = message (node 0) (node 2) (request_vote (node 0) (log_index 0) (election_term 0)) (election_term (Suc 0))) \<and>
+                     log_up_to_date (log (initial_server_state 3)) lastLogIndex lastLogTerm \<and>
+                     (votedFor (initial_server_state 3) = Some (node 0) \<or> votedFor (initial_server_state 3) = None))))
+        (message (node 0) (node 1) (request_vote (node 0) (log_index 0) (election_term 0)) (election_term 1))"
+      apply (simp add: ExReqProps_def initial_server_state_def respond_to_def log_up_to_date_def)
+      by (simp add: less_election_term_def)
 
-    have "[initial_server_state 3\<lparr>currentTerm := election_term (Suc (election_term_of (currentTerm (initial_server_state 3)))), votedFor := Some (node 0)\<rparr>, initial_server_state 3, initial_server_state 3]
-      = [initial_server_state 3\<lparr>currentTerm := election_term (Suc (election_term_of (currentTerm (hd all_states ! 0)))), votedFor := Some (node 0)\<rparr>, initial_server_state 3, initial_server_state 3]"
-      by (simp add: initial_state assms initial_server_state_def repeat_nth)
-    moreover have "hd all_messages \<union> {message (node 0) (node i) (request_vote (node 0) (log_index 0) (election_term 0)) (election_term (Suc (election_term_of (currentTerm (initial_server_state 3))))) | i. i \<le> Suc (Suc 0) \<and> 0 < i}
-      = {message (node 0) (node (Suc 0)) (request_vote (node 0) (log_index 0) (election_term 0)) (election_term (Suc 0)), message (node 0) (node 2) (request_vote (node 0) (log_index 0) (election_term 0)) (election_term (Suc 0))}"
-      apply (simp add: initial_message initial_server_state_def)
+    show "ExReq (message (node (Suc 0)) (node 0) (request_vote_response True) (election_term (Suc 0)))
+     (\<lambda>req. \<not> sender_term req < election_term (Suc (election_term_of (currentTerm (initial_server_state 3)))) \<and>
+             (\<not> sender_term req < election_term (Suc (election_term_of (currentTerm (initial_server_state 3)))) \<longrightarrow>
+              (\<exists>lastLogIndex lastLogTerm.
+                  payload req = request_vote (node 0) lastLogIndex lastLogTerm \<and>
+                  (req = message (node 0) (node (Suc 0)) (request_vote (node 0) (log_index 0) (election_term 0)) (election_term (Suc 0)) \<or>
+                   req = message (node 0) (node 2) (request_vote (node 0) (log_index 0) (election_term 0)) (election_term (Suc 0))) \<and>
+                  log_up_to_date (log (initial_server_state 3)) lastLogIndex lastLogTerm \<and>
+                  (votedFor (initial_server_state 3) = Some (node 0) \<or> votedFor (initial_server_state 3) = None))))"
+      apply (simp add: ExReq_def)
+      using \<open>ExReqProps (message (node (Suc 0)) (node 0) (request_vote_response True) (election_term (Suc 0))) (\<lambda>req. \<not> sender_term req < election_term (Suc (election_term_of (currentTerm (initial_server_state 3)))) \<and> (\<not> sender_term req < election_term (Suc (election_term_of (currentTerm (initial_server_state 3)))) \<longrightarrow> (\<exists>lastLogIndex lastLogTerm. payload req = request_vote (node 0) lastLogIndex lastLogTerm \<and> (req = message (node 0) (node (Suc 0)) (request_vote (node 0) (log_index 0) (election_term 0)) (election_term (Suc 0)) \<or> req = message (node 0) (node 2) (request_vote (node 0) (log_index 0) (election_term 0)) (election_term (Suc 0))) \<and> log_up_to_date (log (initial_server_state 3)) lastLogIndex lastLogTerm \<and> (votedFor (initial_server_state 3) = Some (node 0) \<or> votedFor (initial_server_state 3) = None)))) (message (node 0) (node 1) (request_vote (node 0) (log_index 0) (election_term 0)) (election_term 1))\<close> by blast
+  qed
+  also have "\<dots> \<rightarrow>* (
+    [initial_server_state 3 \<lparr>currentTerm := increment_election_term (currentTerm (initial_server_state 3)), votedFor := Some (node 0)\<rparr>,initial_server_state 3 \<lparr>votedFor := Some (node 0)\<rparr>,initial_server_state 3 \<lparr>votedFor := Some (node 0)\<rparr>],
+    {message (node 2) (node 0) (request_vote_response True) (election_term 1),message (node 1) (node 0) (request_vote_response True) (election_term 1),message (node 0) (node 1) (request_vote (node 0) (log_index 0) (election_term 0)) (election_term 1),message (node 0) (node 2) (request_vote (node 0) (log_index 0) (election_term 0)) (election_term 1)})"
+    apply (rule transitions_one)
+    apply (rule TR_request_vote_resp [where m = 2, where r = 0, where vg = True, where t = "election_term 1", where s = "node 0"])
+    apply (simp add: TR_condition_request_vote_resp_def)
+  proof-
+    have "ExReqProps (message (node 2) (node 0) (request_vote_response True) (election_term (Suc 0)))
+     (\<lambda>req. \<not> sender_term req < election_term (Suc (election_term_of (currentTerm (initial_server_state 3)))) \<and>
+             (\<not> sender_term req < election_term (Suc (election_term_of (currentTerm (initial_server_state 3)))) \<longrightarrow>
+              (\<exists>lastLogIndex lastLogTerm.
+                  payload req = request_vote (node 0) lastLogIndex lastLogTerm \<and>
+                  (req = message (node (Suc 0)) (node 0) (request_vote_response True) (election_term (Suc 0)) \<or>
+                   req = message (node 0) (node (Suc 0)) (request_vote (node 0) (log_index 0) (election_term 0)) (election_term (Suc 0)) \<or>
+                   req = message (node 0) (node 2) (request_vote (node 0) (log_index 0) (election_term 0)) (election_term (Suc 0))) \<and>
+                  log_up_to_date (log (initial_server_state 3)) lastLogIndex lastLogTerm \<and>
+                  (votedFor (initial_server_state 3) = Some (node 0) \<or> votedFor (initial_server_state 3) = None))))
+     (message (node 0) (node 2) (request_vote (node 0) (log_index 0) (election_term 0)) (election_term 1))"
+      apply (simp add: ExReqProps_def initial_server_state_def respond_to_def log_up_to_date_def)
+      by (simp add: less_election_term_def)
+
+    show "ExReq (message (node 2) (node 0) (request_vote_response True) (election_term (Suc 0)))
+     (\<lambda>req. \<not> sender_term req < election_term (Suc (election_term_of (currentTerm (initial_server_state 3)))) \<and>
+             (\<not> sender_term req < election_term (Suc (election_term_of (currentTerm (initial_server_state 3)))) \<longrightarrow>
+              (\<exists>lastLogIndex lastLogTerm.
+                  payload req = request_vote (node 0) lastLogIndex lastLogTerm \<and>
+                  (req = message (node (Suc 0)) (node 0) (request_vote_response True) (election_term (Suc 0)) \<or>
+                   req = message (node 0) (node (Suc 0)) (request_vote (node 0) (log_index 0) (election_term 0)) (election_term (Suc 0)) \<or>
+                   req = message (node 0) (node 2) (request_vote (node 0) (log_index 0) (election_term 0)) (election_term (Suc 0))) \<and>
+                  log_up_to_date (log (initial_server_state 3)) lastLogIndex lastLogTerm \<and>
+                  (votedFor (initial_server_state 3) = Some (node 0) \<or> votedFor (initial_server_state 3) = None)))) \<and>
+    [initial_server_state 3\<lparr>currentTerm := election_term (Suc (election_term_of (currentTerm (initial_server_state 3)))), votedFor := Some (node 0)\<rparr>,
+     initial_server_state 3\<lparr>votedFor := Some (node 0)\<rparr>, initial_server_state 3\<lparr>votedFor := Some (node 0)\<rparr>] =
+    update 2 (initial_server_state 3\<lparr>votedFor := Some (node 0)\<rparr>)
+     [initial_server_state 3\<lparr>currentTerm := election_term (Suc (election_term_of (currentTerm (initial_server_state 3)))), votedFor := Some (node 0)\<rparr>,
+      initial_server_state 3\<lparr>votedFor := Some (node 0)\<rparr>, initial_server_state 3]"
       apply auto
-      done
-    ultimately show "([initial_server_state 3, initial_server_state 3, initial_server_state 3], hd all_messages) \<rightarrow>
-    ([initial_server_state 3\<lparr>currentTerm := election_term (Suc (election_term_of (currentTerm (hd all_states ! 0)))), votedFor := Some (node 0)\<rparr>,
-      initial_server_state 3, initial_server_state 3],
-     {message (node 0) (node (Suc 0)) (request_vote (node 0) (log_index 0) (election_term 0)) (election_term (Suc 0)),
-      message (node 0) (node 2) (request_vote (node 0) (log_index 0) (election_term 0)) (election_term (Suc 0))})"
-      using \<open>([initial_server_state 3, initial_server_state 3, initial_server_state 3], hd all_messages) \<rightarrow> ([initial_server_state 3 \<lparr>currentTerm := election_term (Suc (election_term_of (currentTerm (initial_server_state 3)))), votedFor := Some (node 0)\<rparr>, initial_server_state 3, initial_server_state 3], hd all_messages \<union> {message (node 0) (node i) (request_vote (node 0) (log_index 0) (election_term 0)) (election_term (Suc (election_term_of (currentTerm (initial_server_state 3))))) | i. i \<le> Suc (Suc 0) \<and> 0 < i})\<close> by force
+      using ExReq_def \<open>ExReqProps (message (node 2) (node 0) (request_vote_response True) (election_term (Suc 0))) (\<lambda>req. \<not> sender_term req < election_term (Suc (election_term_of (currentTerm (initial_server_state 3)))) \<and> (\<not> sender_term req < election_term (Suc (election_term_of (currentTerm (initial_server_state 3)))) \<longrightarrow> (\<exists>lastLogIndex lastLogTerm. payload req = request_vote (node 0) lastLogIndex lastLogTerm \<and> (req = message (node (Suc 0)) (node 0) (request_vote_response True) (election_term (Suc 0)) \<or> req = message (node 0) (node (Suc 0)) (request_vote (node 0) (log_index 0) (election_term 0)) (election_term (Suc 0)) \<or> req = message (node 0) (node 2) (request_vote (node 0) (log_index 0) (election_term 0)) (election_term (Suc 0))) \<and> log_up_to_date (log (initial_server_state 3)) lastLogIndex lastLogTerm \<and> (votedFor (initial_server_state 3) = Some (node 0) \<or> votedFor (initial_server_state 3) = None)))) (message (node 0) (node 2) (request_vote (node 0) (log_index 0) (election_term 0)) (election_term 1))\<close> apply blast
+      by (simp add: numeral_2_eq_2)
   qed
   also have "\<dots> \<rightarrow>* (
-    [initial_server_state 3 \<lparr>currentTerm := increment_election_term (currentTerm (hd all_states ! 0)), votedFor := Some (node 0)\<rparr>,
-     initial_server_state 3 \<lparr>votedFor := Some (node 0)\<rparr>, initial_server_state 3],
-    {
-      message (node 0) (node 1) (request_vote (node 0) (log_index 0) (election_term 0)) (election_term 1),
-      message (node 0) (node 2) (request_vote (node 0) (log_index 0) (election_term 0)) (election_term 1),
-      message (node 1) (node 0) (request_vote_response True) (election_term 1)
-    })"
+    [initial_server_state 3 \<lparr>currentTerm := increment_election_term (currentTerm (initial_server_state 3)), votedFor := Some (node 0), state := leader\<rparr>,initial_server_state 3 \<lparr>votedFor := Some (node 0)\<rparr>,initial_server_state 3 \<lparr>votedFor := Some (node 0)\<rparr>],
+    {message (node 2) (node 0) (request_vote_response True) (election_term 1),message (node 1) (node 0) (request_vote_response True) (election_term 1),message (node 0) (node 1) (request_vote (node 0) (log_index 0) (election_term 0)) (election_term 1),message (node 0) (node 2) (request_vote (node 0) (log_index 0) (election_term 0)) (election_term 1)})"
+    (is "\<dots> \<rightarrow>* (?state, ?messages)")
     apply (rule transitions_one)
-    apply (cut_tac TR_request_vote_resp
-        [where \<sigma> = "[initial_server_state 3\<lparr>currentTerm := election_term (Suc (election_term_of (currentTerm (initial_server_state 3)))), votedFor := Some (node 0)\<rparr>, initial_server_state 3, initial_server_state 3]"
-          , where ms = "{ message (node 0) (node 1) (request_vote (node 0) (log_index 0) (election_term 0)) (election_term 1), message (node 0) (node 2) (request_vote (node 0) (log_index 0) (election_term 0)) (election_term 1) }"
-          , where \<sigma>' = "[initial_server_state 3 \<lparr>currentTerm := increment_election_term (currentTerm (hd all_states ! 0)), votedFor := Some (node 0)\<rparr>, initial_server_state 3 \<lparr>votedFor := Some (node 0)\<rparr>, initial_server_state 3]"
-          , where resp = "message (node 1) (node 0) (request_vote_response True) (election_term 1)"
-          , where s = "node 0"
-          ])
-    apply simp_all
-    apply (simp add: assms initial_state insert_commute numeral_3_eq_3)
-    defer
-    apply (simp add: initial_state assms initial_server_state_def repeat_nth)
-    apply simp
-    apply (simp add: ExReq_def initial_state initial_server_state_def)
+    apply (rule TR_promote_to_leader [where target = 0])
+    apply (simp add: TR_condition_promote_to_leader_def)
+    apply (simp add: majority_def initial_server_state_def)
   proof-
-    have "\<And>req. req = message (node 0) (node 1) (request_vote (node 0) (log_index 0) (election_term 0)) (election_term 1)
-      \<Longrightarrow> \<not> sender_term req < election_term (Suc 0) \<and>
-          (\<not> sender_term req < election_term (Suc 0) \<longrightarrow>
-           (\<exists>lastLogIndex lastLogTerm.
-               payload req = request_vote (node 0) lastLogIndex lastLogTerm \<and>
-               (req = message (node 0) (node (Suc 0)) (request_vote (node 0) (log_index 0) (election_term 0)) (election_term (Suc 0)) \<or>
-                req = message (node 0) (node 2) (request_vote (node 0) (log_index 0) (election_term 0)) (election_term (Suc 0))) \<and>
-               log_up_to_date [] lastLogIndex lastLogTerm)) \<and>
-          respond_to (message (node (Suc 0)) (node 0) (request_vote_response True) (election_term (Suc 0))) req"
-      apply (auto simp add: respond_to_def)
-      using less_election_term_def apply force
-      apply (simp add: log_up_to_date_def)
-      done
-    show "\<exists>req. \<not> sender_term req < election_term (Suc 0) \<and>
-          (\<not> sender_term req < election_term (Suc 0) \<longrightarrow>
-           (\<exists>lastLogIndex lastLogTerm.
-               payload req = request_vote (node 0) lastLogIndex lastLogTerm \<and>
-               (req = message (node 0) (node (Suc 0)) (request_vote (node 0) (log_index 0) (election_term 0)) (election_term (Suc 0)) \<or>
-                req = message (node 0) (node 2) (request_vote (node 0) (log_index 0) (election_term 0)) (election_term (Suc 0))) \<and>
-               log_up_to_date [] lastLogIndex lastLogTerm)) \<and>
-          respond_to (message (node (Suc 0)) (node 0) (request_vote_response True) (election_term (Suc 0))) req"
-      by (meson \<open>\<And>req. req = message (node 0) (node 1) (request_vote (node 0) (log_index 0) (election_term 0)) (election_term 1) \<Longrightarrow> \<not> sender_term req < election_term (Suc 0) \<and> (\<not> sender_term req < election_term (Suc 0) \<longrightarrow> (\<exists>lastLogIndex lastLogTerm. payload req = request_vote (node 0) lastLogIndex lastLogTerm \<and> (req = message (node 0) (node (Suc 0)) (request_vote (node 0) (log_index 0) (election_term 0)) (election_term (Suc 0)) \<or> req = message (node 0) (node 2) (request_vote (node 0) (log_index 0) (election_term 0)) (election_term (Suc 0))) \<and> log_up_to_date [] lastLogIndex lastLogTerm)) \<and> respond_to (message (node (Suc 0)) (node 0) (request_vote_response True) (election_term (Suc 0))) req\<close>)
-  qed
-  also have "\<dots> \<rightarrow>* (
-    [initial_server_state 3 \<lparr>currentTerm := increment_election_term (currentTerm (hd all_states ! 0)), votedFor := Some (node 0)\<rparr>,
-     initial_server_state 3 \<lparr>votedFor := Some (node 0)\<rparr>,
-     initial_server_state 3 \<lparr>votedFor := Some (node 0)\<rparr>],
-    {
-      message (node 0) (node 1) (request_vote (node 0) (log_index 0) (election_term 0)) (election_term 1),
-      message (node 0) (node 2) (request_vote (node 0) (log_index 0) (election_term 0)) (election_term 1),
-      message (node 1) (node 0) (request_vote_response True) (election_term 1),
-      message (node 2) (node 0) (request_vote_response True) (election_term 1)
-    })"
-    apply (rule transitions_one)
-    apply (cut_tac TR_request_vote_resp
-        [where \<sigma> = "[initial_server_state 3 \<lparr>currentTerm := increment_election_term (currentTerm (hd all_states ! 0)), votedFor := Some (node 0)\<rparr>, initial_server_state 3 \<lparr>votedFor := Some (node 0)\<rparr>, initial_server_state 3]"
-          , where ms = "{message (node 0) (node 1) (request_vote (node 0) (log_index 0) (election_term 0)) (election_term 1),message (node 0) (node 2) (request_vote (node 0) (log_index 0) (election_term 0)) (election_term 1),message (node 1) (node 0) (request_vote_response True) (election_term 1)}"
-          , where \<sigma>' = "[initial_server_state 3 \<lparr>currentTerm := increment_election_term (currentTerm (hd all_states ! 0)), votedFor := Some (node 0)\<rparr>,initial_server_state 3 \<lparr>votedFor := Some (node 0)\<rparr>,initial_server_state 3 \<lparr>votedFor := Some (node 0)\<rparr>]"
-          , where resp = "message (node 2) (node 0) (request_vote_response True) (election_term 1)"
-          , where s = "node 0"
-          ])
-    apply simp_all
-    apply (simp add: assms initial_state insert_commute numeral_3_eq_3)
-    defer
-    apply (simp add: initial_state assms initial_server_state_def repeat_nth numeral_2_eq_2)
-    apply simp
-    apply (simp add: ExReq_def initial_state initial_server_state_def)
-  proof-
-    have "\<And>req. req = message (node 0) (node 2) (request_vote (node 0) (log_index 0) (election_term 0)) (election_term 1)
-      \<Longrightarrow>\<not> sender_term req
-             < election_term
-                (Suc (election_term_of
-                       (currentTerm
-                         (repeat
-                           \<lparr>state = follower, currentTerm = election_term 0, votedFor = None, log = [], commitIndex = 0, lastApplied = 0,
-                              nextIndex = repeat (log_index 0) number_of_nodes, matchIndex = repeat (log_index 0) number_of_nodes\<rparr>
-                           number_of_nodes !
-                          0)))) \<and>
-          (\<not> sender_term req
-              < election_term
-                 (Suc (election_term_of
-                        (currentTerm
-                          (repeat
-                            \<lparr>state = follower, currentTerm = election_term 0, votedFor = None, log = [], commitIndex = 0, lastApplied = 0,
-                               nextIndex = repeat (log_index 0) number_of_nodes, matchIndex = repeat (log_index 0) number_of_nodes\<rparr>
-                            number_of_nodes !
-                           0)))) \<longrightarrow>
-           (\<exists>lastLogIndex lastLogTerm.
-               payload req = request_vote (node 0) lastLogIndex lastLogTerm \<and>
-               (req = message (node 0) (node (Suc 0)) (request_vote (node 0) (log_index 0) (election_term 0)) (election_term (Suc 0)) \<or>
-                req = message (node 0) (node 2) (request_vote (node 0) (log_index 0) (election_term 0)) (election_term (Suc 0)) \<or>
-                req = message (node (Suc 0)) (node 0) (request_vote_response True) (election_term (Suc 0))) \<and>
-               log_up_to_date [] lastLogIndex lastLogTerm)) \<and>
-          respond_to (message (node 2) (node 0) (request_vote_response True) (election_term (Suc 0))) req"
-      apply (auto simp add: respond_to_def assms repeat_nth)
-      using less_election_term_def apply force
-      apply (simp add: log_up_to_date_def)
-      done
-    show "\<exists>req. \<not> sender_term req
-             < election_term
-                (Suc (election_term_of
-                       (currentTerm
-                         (repeat
-                           \<lparr>state = follower, currentTerm = election_term 0, votedFor = None, log = [], commitIndex = 0, lastApplied = 0,
-                              nextIndex = repeat (log_index 0) number_of_nodes, matchIndex = repeat (log_index 0) number_of_nodes\<rparr>
-                           number_of_nodes !
-                          0)))) \<and>
-          (\<not> sender_term req
-              < election_term
-                 (Suc (election_term_of
-                        (currentTerm
-                          (repeat
-                            \<lparr>state = follower, currentTerm = election_term 0, votedFor = None, log = [], commitIndex = 0, lastApplied = 0,
-                               nextIndex = repeat (log_index 0) number_of_nodes, matchIndex = repeat (log_index 0) number_of_nodes\<rparr>
-                            number_of_nodes !
-                           0)))) \<longrightarrow>
-           (\<exists>lastLogIndex lastLogTerm.
-               payload req = request_vote (node 0) lastLogIndex lastLogTerm \<and>
-               (req = message (node 0) (node (Suc 0)) (request_vote (node 0) (log_index 0) (election_term 0)) (election_term (Suc 0)) \<or>
-                req = message (node 0) (node 2) (request_vote (node 0) (log_index 0) (election_term 0)) (election_term (Suc 0)) \<or>
-                req = message (node (Suc 0)) (node 0) (request_vote_response True) (election_term (Suc 0))) \<and>
-               log_up_to_date [] lastLogIndex lastLogTerm)) \<and>
-          respond_to (message (node 2) (node 0) (request_vote_response True) (election_term (Suc 0))) req"
-      by (meson \<open>\<And>req. req = message (node 0) (node 2) (request_vote (node 0) (log_index 0) (election_term 0)) (election_term 1) \<Longrightarrow> \<not> sender_term req < election_term (Suc (election_term_of (currentTerm (repeat \<lparr>state = follower, currentTerm = election_term 0, votedFor = None, log = [], commitIndex = 0, lastApplied = 0, nextIndex = repeat (log_index 0) number_of_nodes, matchIndex = repeat (log_index 0) number_of_nodes\<rparr> number_of_nodes ! 0)))) \<and> (\<not> sender_term req < election_term (Suc (election_term_of (currentTerm (repeat \<lparr>state = follower, currentTerm = election_term 0, votedFor = None, log = [], commitIndex = 0, lastApplied = 0, nextIndex = repeat (log_index 0) number_of_nodes, matchIndex = repeat (log_index 0) number_of_nodes\<rparr> number_of_nodes ! 0)))) \<longrightarrow> (\<exists>lastLogIndex lastLogTerm. payload req = request_vote (node 0) lastLogIndex lastLogTerm \<and> (req = message (node 0) (node (Suc 0)) (request_vote (node 0) (log_index 0) (election_term 0)) (election_term (Suc 0)) \<or> req = message (node 0) (node 2) (request_vote (node 0) (log_index 0) (election_term 0)) (election_term (Suc 0)) \<or> req = message (node (Suc 0)) (node 0) (request_vote_response True) (election_term (Suc 0))) \<and> log_up_to_date [] lastLogIndex lastLogTerm)) \<and> respond_to (message (node 2) (node 0) (request_vote_response True) (election_term (Suc 0))) req\<close>)
-  qed
-  also have "\<dots> \<rightarrow>* (
-    [initial_server_state 3 \<lparr>currentTerm := increment_election_term (currentTerm (hd all_states ! 0)), votedFor := Some (node 0), state := leader\<rparr>,
-     initial_server_state 3 \<lparr>votedFor := Some (node 0)\<rparr>,
-     initial_server_state 3 \<lparr>votedFor := Some (node 0)\<rparr>],
-    {
-      message (node 0) (node 1) (request_vote (node 0) (log_index 0) (election_term 0)) (election_term 1),
-      message (node 0) (node 2) (request_vote (node 0) (log_index 0) (election_term 0)) (election_term 1),
-      message (node 1) (node 0) (request_vote_response True) (election_term 1),
-      message (node 2) (node 0) (request_vote_response True) (election_term 1)
-    })" (is "\<dots> \<rightarrow>* (?state, ?messages)")
-    apply (rule transitions_one)
-    apply (cut_tac TR_promote_to_leader
-        [where \<sigma> = "[initial_server_state 3 \<lparr>currentTerm := increment_election_term (currentTerm (hd all_states ! 0)), votedFor := Some (node 0)\<rparr>,initial_server_state 3 \<lparr>votedFor := Some (node 0)\<rparr>,initial_server_state 3 \<lparr>votedFor := Some (node 0)\<rparr>]"
-          , where ms = "{message (node 0) (node 1) (request_vote (node 0) (log_index 0) (election_term 0)) (election_term 1),message (node 0) (node 2) (request_vote (node 0) (log_index 0) (election_term 0)) (election_term 1),message (node 1) (node 0) (request_vote_response True) (election_term 1),message (node 2) (node 0) (request_vote_response True) (election_term 1)}"
-          , where target = "0"
-          , where \<sigma>' = "[initial_server_state 3 \<lparr>currentTerm := increment_election_term (currentTerm (hd all_states ! 0)), votedFor := Some (node 0), state := leader\<rparr>,initial_server_state 3 \<lparr>votedFor := Some (node 0)\<rparr>,initial_server_state 3 \<lparr>votedFor := Some (node 0)\<rparr>]"
-          ])
-    apply simp_all
-    apply (simp add: assms majority_def initial_state initial_server_state_def repeat_nth)
-  proof-
-    have "{s. s = node 1 \<or> s = node 2} = {node 1, node 2}"
+    have "{s. s = node 2 \<or> s = node (Suc 0)} = {node 1, node 2}"
       by auto
     moreover have "node 1 \<noteq> node 2"
       by simp
-    ultimately have "card {s. s = node 1 \<or> s = node 2} = 2"
+    ultimately have "card {s. s = node 2 \<or> s = node (Suc 0)} = 2"
       by simp
-    thus "Suc (Suc (Suc 0)) < 2 * card {s. s = node (Suc 0) \<or> s = node 2}"
+    thus "Suc (Suc (Suc 0)) < 2 * card {s. s = node 2 \<or> s = node (Suc 0)}"
       by simp
   qed
   finally have "(hd all_states, hd all_messages) \<rightarrow>* (?state, ?messages)" "state (?state ! 0) = leader"
